init VC lecture

code/Cse230wi25/full/L08VerificationConditions.lean
@@ -1,38 +1,56 @@
-import LeanConcreteSemantics.BigStep
-import LeanConcreteSemantics.Ch12Axiomatic
-
-import Smt
+import Cse230wi25.BigStep
+import Cse230wi25.L07Axiomatic
 
 set_option pp.fieldNotation false
 set_option pp.proofs true
+
+/- @@@
+
+# Automating Floyd-Hoare with Verification Conditions
+
+FH rules are nice but still *quite* tedious to use, because it seems like we
+need to spell out
+
+1. where to apply which rule
+2. how exactly the rules of consequence work
+
+etc.
+
+In fact, the rules are *mostly* **syntax directed** meaning that there is
+**exactly one** rule that can be applied for each kind of term.
+
+- The rules of _consequence_
+- The loop _invariant_
+
+Next, lets see how we can automate away more or less everything except
+the above.
+
+@@@ -/
+
+/- @@@
+
+## Annotated Commands
+
+Lets assume that the programmer has **annotated** their code with the
+loop invariant, so we can define a `ACom` type which looks just like
+the previous `Com` except for the loop constructor which is now of the
+form `While inv b c` case, so the `inv` is baked into the code.
+
+@@@ -/
+
 
 inductive ACom where
   | Skip   : ACom
   | Assign : Vname -> Aexp -> ACom
   | Seq    : ACom  -> ACom -> ACom
   | If     : Bexp  -> ACom -> ACom -> ACom
-  | While  : Assn -> Bexp  -> ACom -> ACom
+  | While  : Assertion -> Bexp  -> ACom -> ACom
 open ACom
 
-@[simp]
-def pre (c: ACom) (q : Assn) : Assn :=
-  match c with
-  | ACom.Skip        => q
-  | ACom.Assign x a  => ( q [[ x := a ]] )
-  | ACom.Seq c1 c2   => pre c1 (pre c2 q)
-  | ACom.If b c1 c2  => (λ s => if bval b s then pre c1 q s else pre c2 q s)
-  | ACom.While i _ _ => i
-
-@[simp]
-def vc (c : ACom) (q : Assn) : Prop :=
-  match c with
-  | ACom.Skip        => True
-  | ACom.Assign _ _  => True
-  | ACom.Seq c1 c2   => vc c1 (pre c2 q) /\ (vc c2 q)
-  | ACom.If _ c1 c2  => vc c1 q /\ vc c2 q
-  | ACom.While i b c => (∀ s, i s -> bval b s -> pre c i s) /\
-                        (∀ s, i s -> ¬ bval b s -> q s) /\
-                        vc c i
+/- @@@
+In fact, if we `erase` the `inv` from each while, we can convert an `ACom` program
+back into the old `Com` programs.
+@@@ -/
 
 @[simp]
 def erase (c : ACom) : Com :=
@@ -43,35 +61,10 @@ def erase (c : ACom) : Com :=
   | ACom.If b c1 c2  => Com.If b    (erase c1) (erase c2)
   | ACom.While _ b c => Com.While b (erase c)
 
+/- @@@
+As before we can define some "notation" to make it easier to write `ACom` programs.
+@@@ -/
 
-
-theorem vc_sound : vc c q -> (⊢ {{ pre c q }} (erase c) {{ q }})
-  := by
-  intros vcq
-  induction c generalizing q
-  . case Skip   => constructor
-  . case Assign => constructor
-  . case Seq 	=> sorry
-  . case If 	=> sorry 
-  . case While 	=> sorry
-
-/- ----------------------------------------------------------------------------------------------- -/
-
-@[simp]
-def vc' (p: Assn) (c: ACom) (q: Assn) : Prop := (p ⊆ pre c q) ∧ (vc c q)
-
-theorem vc'_sound : vc' p c q -> (⊢ {{ p }} (erase c) {{ q }}) := by
-  intros vcq
-  cases vcq
-  rename_i vc1 vc2
-  apply FH.Cnsq
-  apply vc1
-  apply vc_sound; assumption
-  apply implies_refl
-
-
-/- ----------------------------------------------------------------------------------------------- -/
--- use `notation` for the below
 notation:10 x "<~" e  => ACom.Assign x (ToAexp.toAexp e)
 infixr:20 ";;"  => ACom.Seq
 notation:10 "IF" b "THEN" c1 "ELSE" c2 => ACom.If b c1 c2
@@ -79,11 +72,65 @@ notation:12 "WHILE {-@" inv "@-}" b "DO" c "END" => ACom.While inv (ToBexp.toBex
 notation:20 "[|" c "|]" => erase c
 notation:10 "⊢" " {|" p "|}" c "{|" q "|}" => FH p (erase c) q
 
-@[simp]
-def tt : Assn := λ_ => True
+/- @@@
+
+Specifically, note the `⊢ {| p |} c {| q |}` triple
+which means that the triple holds for the **erased**
+command `c`.
+
+## Weakest Preconditions
+
+The central idea is reformulate the FH rules into the notion
+of the **weakest precondition** `wp c q` which defines the
+**largest** set of *starting states* from which executing
+the command `c` will yield a *final state* in which the
+assertion `q` is guaranteed to hold.
+
+@@@ -/
 
 @[simp]
-def ff : Assn := λ_ => False
+def wp (c: ACom) (q : Assertion) : Assertion :=
+  match c with
+  | ACom.Skip        => q
+  | ACom.Assign x a  => q [[ x := a ]]
+  | ACom.Seq c1 c2   => wp c1 (wp c2 q)
+  | ACom.If b c1 c2  => (λ s => if bval b s then wp c1 q s else wp c2 q s)
+  | ACom.While i _ _ => i
+
+@[simp]
+def vc (c : ACom) (q : Assertion) : Prop :=
+  match c with
+  | ACom.Skip        => True
+  | ACom.Assign _ _  => True
+  | ACom.Seq c1 c2   => vc c1 (wp c2 q) /\ (vc c2 q)
+  | ACom.If _ c1 c2  => vc c1 q /\ vc c2 q
+  | ACom.While i b c => (∀ s, i s -> bval b s -> wp c i s) /\
+                        (∀ s, i s -> ¬ bval b s -> q s) /\
+                        vc c i
+
+theorem vc_sound : vc c q -> (⊢ {{ wp c q }} (erase c) {{ q }})
+  := by
+  intros vcq
+  induction c generalizing q
+  . case Skip   => constructor
+  . case Assign => constructor
+  . case Seq => sorry
+  . case If => sorry
+  . case While => sorry
+
+/- ----------------------------------------------------------------------------------------------- -/
+
+@[simp]
+def vc' (p: Assertion) (c: ACom) (q: Assertion) : Prop := (p ⊆ wp c q) ∧ (vc c q)
+
+theorem vc'_sound : vc' p c q -> (⊢ {{ p }} (erase c) {{ q }}) := by
+  intros vcq
+  cases vcq
+  rename_i vc1 vc2
+  apply FH.CnsL
+  apply vc_sound; assumption
+  apply vc1
+
 
 theorem ex1 : ⊢ {| tt |}
                   x <~ 5
@@ -98,11 +145,11 @@ theorem ex2 : ⊢ {| λs => s x = 10 |}
   := by
   apply vc'_sound; simp_all [aval, upd]
 
-theorem ex3 : ⊢ {| λs => s x = a /\ s y = b |}
+theorem ex_swap : ⊢ {| λs => s x = a /\ s y = b |}
                     (z <~ x) ;;
                     (x <~ y) ;;
                     (y <~ z)
-                {| λs => s x = b /\ s y = a |}
+                    {| λs => s x = b /\ s y = a |}
   := by
   apply vc'_sound; simp_all [aval, upd]
 
@@ -114,6 +161,24 @@ theorem ex4 : ⊢ {| tt |}
   := by
   apply vc'_sound
   simp_all [aval, bval]
+
+theorem ex_loop : ⊢ {| tt |}
+                    (y <~ 0)
+                    ;;
+                    (x <~ 100)
+                    ;;
+                    (WHILE {-@ λ s => 100 <= s x /\ 0 <= s y @-} y << z DO
+                       ((x <~ x + y) ;;
+                        (y <~ y - 1))
+                    END)
+                    {| λ s => 100 <= s x |}
+  := by
+  apply vc'_sound
+  simp_all [aval, bval, upd]
+  intros s hx _
+  calc 100 <= s x       := by assumption
+       _   <= s x + s y := by simp_arith []
+
 
 theorem imp_sum' : ⊢ {| λ s => s "x" = i |}
                       (y <~ 0) ;;
@@ -136,9 +201,3 @@ theorem imp_sum' : ⊢ {| λ s => s "x" = i |}
     rename_i s _ _
     generalize hx : s x = vx
     cases vx <;> simp_all [sum, Nat.add_assoc]
-
-/- SMT stuff ------------------------------------------------------------------------------------- -/
-example {U : Type} [Nonempty U] {f : U → U → U} {a b c d : U}
-  (h0 : a = b) (h1 : c = d) (h2 : p1 ∧ True) (h3 : (¬ p1) ∨ (p2 ∧ p3))
-  (h4 : (¬ p3) ∨ (¬ (f a c = f b d))) : False := by
-  smt [h0, h1, h2, h3, h4]
