code/Cse230wi25/Arith.lean
@@ -1,0 +1,2 @@
+
+def inc(x:Nat) := x + 1
