src/lectures/Arith.md
@@ -1,0 +1,5 @@
+
+```lean
+def inc(x:Nat) := x + 1
+```
+
