src/lectures/BigStep.md
@@ -1,0 +1,39 @@
+```lean
+import Cse230wi25.States
+import Cse230wi25.IMP
+
+open Com
+
+-- inductive BigStep : Com -> State -> State -> Prop where
+--   | Skip {st} :  BigStep Skip st st
+--   | Assign {st a n} : BigStep (Assign a n) st (st [a := aval n st])
+--   | Seq {c1 c2 st1 st2 st3} : BigStep c1 st1 st2 -> BigStep c2 st2 st3 -> BigStep (Seq c1 c2) st1 st3
+--   | IfTrue {b c1 c2 st st'} : bval b st = true -> BigStep c1 st st' -> BigStep (If b c1 c2) st st'
+--   | IfFalse {b c1 c2 st st'} : bval b st = false -> BigStep c2 st st' -> BigStep (If b c1 c2) st st'
+--   | WhileFalse {b c st} : bval b st = false -> BigStep (While b c) st st
+--   | WhileTrue {b c st st' st''} : bval b st = true -> BigStep c st st' -> BigStep (While b c) st' st'' -> BigStep (While b c) st st''
+
+inductive BigStep : Com -> State -> State -> Prop where
+  | Skip   : ∀ {st},
+                BigStep Skip st st
+  | Assign : ∀ {st a n},
+                BigStep (Assign a n) st (st [a := aval n st])
+  | Seq    : ∀ {c1 c2 st1 st2 st3},
+                BigStep c1 st1 st2 -> BigStep c2 st2 st3 ->
+                BigStep (Seq c1 c2) st1 st3
+  | IfTrue : ∀ {b c1 c2 st st'},
+                bval b st = true -> BigStep c1 st st' ->
+                BigStep (If b c1 c2) st st'
+  | IfFalse : ∀ {b c1 c2 st st'},
+                bval b st = false -> BigStep c2 st st' ->
+                BigStep (If b c1 c2) st st'
+  | WhileFalse : ∀ {b c st},
+                bval b st = false ->
+                BigStep (While b c) st st
+  | WhileTrue : ∀ {b c st st' st''},
+                bval b st = true -> BigStep c st st' -> BigStep (While b c) st' st'' ->
+                BigStep (While b c) st st''
+
+notation:12 "⟨" c "," s "⟩ ==> " t  => BigStep c s t
+```
+
