src/lectures/Expressions.md
@@ -1,0 +1,151 @@
+```lean
+import Cse230wi25.States
+
+set_option pp.fieldNotation false
+set_option pp.proofs true
+
+
+-- Arithmetic Expressions -------------------------------------
+
+inductive Aexp where
+  | num : Val -> Aexp
+  | var : Vname -> Aexp
+  | add : Aexp -> Aexp -> Aexp
+  | sub : Aexp -> Aexp -> Aexp
+  deriving Repr
+
+open Aexp
+
+class ToAexp (a : Type) where
+  toAexp : a -> Aexp
+
+instance : ToAexp Nat where
+  toAexp := num
+
+instance : ToAexp String where
+  toAexp := var
+
+instance : ToAexp Aexp where
+  toAexp a := a
+
+instance : OfNat Aexp (n: Nat) where
+  ofNat := num n
+
+instance : Add Aexp where
+  add := fun a1 a2 => add a1 a2
+
+-- instance [ToAexp a] [ToAexp b] : HAdd a b Aexp where
+--   hAdd := fun s a => .Add (ToAexp.toAexp s) (ToAexp.toAexp a)
+
+instance : HAdd String Aexp Aexp where
+   hAdd := fun s a => add (var s) a
+
+instance : HAdd String Nat Aexp where
+   hAdd := fun s a => add (var s) (num a)
+
+instance : HAdd String String Aexp where
+   hAdd := fun s a => add (var s) (var a)
+
+instance : HSub String Nat Aexp where
+   hSub := fun s a => sub (var s) (num a)
+
+
+def mkVar (s: String) (i : Nat) : Aexp := var (s!"{s}_{i}")
+
+notation:80 lhs:91 "#" rhs:90 => mkVar lhs rhs
+
+@[simp]
+def x := "x"
+
+@[simp]
+def y := "y"
+
+@[simp]
+def z := "z"
+
+def aexp0 : Aexp := x#1 + y#1 + z#1 + 5
+
+def aval (a: Aexp) (s: State) : Val :=
+  match a with
+  | num n => n
+  | var x => s x
+  | add a1 a2 => aval a1 s + aval a2 s
+  | sub a1 a2 => aval a1 s - aval a2 s
+
+-- initial state
+def st0 : State := λ _ => 0
+def aexp_5 := num 5
+def aexp_x := var "x"
+def aexp_x_plus_y := add (var "x") (var "y")
+def aexp_2_plus_z_plus_3 := add (num 2) (add (var "z") (num 3))
+
+-- Substitution -----------------------------------------------
+
+def subst (x : Vname) (xa : Aexp) (a : Aexp) : Aexp :=
+  match a with
+  | num n => num n
+  | var y => if x = y then xa else var y
+  | add a1 a2 => add (subst x xa a1) (subst x xa a2)
+  | sub a1 a2 => sub (subst x xa a1) (subst x xa a2)
+
+example : subst "x" (num 3) (add (var "x") (var "y")) = add (num 3) (var "y") := rfl
+
+theorem subst_aval : ∀ {x xa a}, aval (subst x xa a) s = aval a (s [x := aval xa s])
+  := by
+  intros x xa a
+  induction a
+  case num n => simp [subst, aval]
+  case var y => simp [subst, aval]
+                split
+                case isTrue => simp [upd, *]
+                case isFalse => simp [upd, *]; split <;> simp_all [aval]
+  case add a1 a2 ih1 ih2 => simp_all [subst, aval]
+  case sub a1 a2 ih1 ih2 => simp_all [subst, aval]
+
+
+-- Boolean Expressions ---------------------------------------------
+
+inductive Bexp where
+  | Bc    : Bool -> Bexp
+  | Bnot  : Bexp -> Bexp
+  | Band  : Bexp -> Bexp -> Bexp
+  | BLess : Aexp -> Aexp -> Bexp
+  deriving Repr
+
+open Bexp
+
+class ToBexp (a : Type) where
+  toBexp : a -> Bexp
+
+@[simp]
+instance : ToBexp Bool where
+  toBexp := Bc
+
+@[simp]
+instance : ToBexp Bexp where
+  toBexp (b) := b
+
+
+def bval (b: Bexp) (st: State) : Bool :=
+  match b with
+  | Bc v        => v
+  | Bnot b1     => ! bval b1 st
+  | Band b1 b2  => bval b1 st && bval b2 st
+  | BLess a1 a2 => aval a1 st < aval a2 st
+
+def bsubst (x : Vname) (xa : Aexp) (b : Bexp) : Bexp :=
+  match b with
+  | Bc v        => Bc v
+  | Bnot b'     => Bnot  (bsubst x xa b')
+  | Band  b1 b2 => Band  (bsubst x xa b1) (bsubst x xa b2)
+  | BLess a1 a2 => BLess (subst x xa a1) (subst x xa a2)
+
+theorem subst_bval : ∀ {x xa b}, bval (bsubst x xa b) s = bval b (s [x := aval xa s]) := by
+  intros x xa b
+  induction b
+  case Bc v       => simp_all [bsubst, bval]
+  case Bnot b' ih => simp_all [bsubst, bval, ih]
+  case Band b1 b2 ih1 ih2 => simp_all [bsubst, bval, ih1, ih2]
+  case BLess a1 a2 => simp_all [bsubst, bval, subst_aval]
+```
+
