src/lectures/IMP.md
@@ -1,0 +1,41 @@
+```lean
+import Cse230wi25.States
+import Cse230wi25.Expressions
+
+set_option pp.fieldNotation false
+set_option pp.proofs true
+
+-- Commands ----------------------------------------------------------
+
+inductive Com where
+  | Skip   : Com
+  | Assign : Vname -> Aexp -> Com
+  | Seq    : Com   -> Com  -> Com
+  | If     : Bexp  -> Com  -> Com -> Com
+  | While  : Bexp  -> Com  -> Com
+  deriving Repr
+
+open Com
+
+def bLess (a1 a2 : Aexp) : Bexp := Bexp.BLess a1 a2
+
+infix:10 "<<"  => fun x y => Bexp.BLess (ToAexp.toAexp x) (ToAexp.toAexp y)
+infix:10 "<~"  => Com.Assign
+infixr:8 ";;"  => Com.Seq
+notation:10 "IF" b "THEN" c1 "ELSE" c2 => Com.If b c1 c2
+notation:12 "WHILE" b "DO" c "END" => Com.While b c
+
+def com0 := "x" <~ "y" + 1
+def com1 := "y" <~ 2
+def com2 := com0 ;; com1
+def com3 := x <~ y + 1 ;; y <~ x + 2
+def com4 := Skip ;; Skip ;; Skip ;; Skip
+def com5 := IF 10 << x THEN x <~ 1 ELSE y <~ 2
+def com6 := WHILE x << 5 DO x <~ x + 1 END
+
+def st_x_10_y_20 := st0 [x := 10 ] [ y := 20]
+
+#eval com3
+#eval com4
+```
+
