src/lectures/L03Induction_lec.md
@@ -1,0 +1,153 @@
+```lean
+set_option pp.fieldNotation false
+```
+
+# Datatypes and Recursion
+
+This material is based on
+
+- Chapter 2 of [Concrete Semantics](http://www.concrete-semantics.org/)
+- Induction Exercises by [James Wilcox](https://jamesrwilcox.com/InductionExercises.html)
+
+
+```lean
+namespace MyNat
+
+inductive Nat where
+  | zero : Nat
+  | succ : Nat -> Nat
+  deriving Repr
+
+open Nat
+
+def add (n m : Nat) : Nat :=
+  match n with
+  | zero => m
+  | succ n' => succ (add n' m)
+```
+
+## Trick 1: Helper Lemmas
+
+
+### Helper Lemmas: Example `add_comm`
+
+
+```lean
+theorem add_zero : ∀ (m : Nat),
+  add m zero = m := by
+  intros m
+  induction m
+  . case zero =>
+    rfl
+  . case succ m' ih =>
+    simp [add, ih]
+
+theorem add_succ : ∀ (m n : Nat),
+  add m (succ n) = succ (add m n) := by
+  intros m n
+  induction m
+  . case zero => rfl
+  . case succ m' ih =>
+    simp [add, *]
+
+theorem add_comm : ∀ (n m: Nat),
+  add n m = add m n := by
+  intros n m
+  induction n
+  . case zero =>
+    simp [add, add_zero]
+  . case succ n' ih =>
+    simp [add, add_succ, *]
+
+
+
+
+
+
+
+end MyNat
+```
+
+### Helper Lemmas: Example `rev_rev`
+
+```lean
+open List
+```
+
+**Appending lists**
+
+```lean
+def app {α : Type} (xs ys: List α) : List α :=
+  match xs with
+  | [] => ys
+  | x::xs' => x :: app xs' ys
+
+example : app [0,1,2] [3,4,5] = [0,1,2,3,4,5] := rfl
+```
+
+**Reversing lists**
+
+```lean
+def rev {α : Type} (xs: List α) : List α :=
+  match xs with
+  | [] => []
+  | x :: xs' => app (rev xs') [x]
+
+example : rev [0,1,2,3] = [3,2,1,0] := rfl
+
+------- CUT -----
+
+theorem rev_rev : ∀ {α : Type} (xs: List α),
+  rev (rev xs) = xs := by
+  sorry
+```
+
+
+## Trick 2: Generalizing
+
+```lean
+open MyNat.Nat
+
+def itadd (n m: MyNat.Nat) : MyNat.Nat :=
+  match n with
+  | zero => m
+  | succ n' => itadd n' (succ m)
+
+theorem itadd_eq : ∀ (n m: MyNat.Nat), itadd n m = MyNat.add n m := by
+  sorry
+
+open List
+
+def itrev {α : Type} (xs ys: List α) : List α :=
+  match xs with
+  | [] => ys
+  | x ::xs' => itrev xs' (x :: ys)
+
+theorem itrev_eq_rev : ∀ {α : Type} (xs: List α), itrev xs [] = rev xs := by
+  sorry
+```
+
+
+## Trick 3: Functional Induction
+
+Based on [Joachim Breitner's notes on Functional Induction](https://lean-lang.org/blog/2024-5-17-functional-induction/)
+
+
+```lean
+def len (xs: List α) : Nat :=
+  match xs with
+  | [] => 0
+  | _::xs' => 1 + len xs'
+
+def alt (xs ys : List α) : List α :=
+  match xs, ys with
+  | [], ys => ys
+  | xs, [] => xs
+  | x::xs, y::ys => x :: y :: alt xs ys
+
+#eval alt [1,2,3,4] [10,20,30]
+
+theorem alt_length : ∀ {α : Type} (xs ys : List α), len (alt xs ys) = len xs + len ys := by
+  sorry
+```
+
