src/lectures/L07Axiomatic.md
@@ -1,0 +1,995 @@
+```lean
+import Cse230wi25.BigStep
+
+set_option pp.fieldNotation false
+set_option pp.proofs true
+```
+
+
+# Axiomatic Semantics
+
+The `BigStep` semantics that was saw previously was helpful in proving properties
+about **groups** of programs, for example, that
+
+1. that *every* command `c` was **deterministic** or
+2. that *every* command `c` was **equivalent to** `SKIP ;; c` or `IF cond THEN c ELSE c` or
+3. that *every* command `x <~ a;; y <~ a` was equivalent to `x <~ a;; y <~ x` (if `x` was not read in `a`).
+
+Next, lets try to use the `BigStep` semantics to check properties of **individual** programs.
+
+
+## Example: Swapping two Variables
+
+Consider the following `Com` program that *swaps*
+the values of `x` and `y` using `z` as a temporary
+storage.
+
+
+```lean
+open Aexp
+
+def swap :=
+
+-- {{ y = b /\ x = a }}
+
+  z <~ var x ;;
+
+-- {{ y = b /\ z = a }}
+
+  x <~ var y ;;
+
+-- {{ x = b /\ z = a }}
+
+  y <~ var z
+
+-- {{ x = b /\ y = a }}
+
+
+theorem swap_ok : ∀ {s t a b},
+  (⟨ swap , s ⟩ ==> t) ->
+  (s x = a /\ s y = b) ->
+  (t x = b /\ t y = a) := by
+  intros s t a b swap_s_t xa_yb
+  simp_all [swap]
+  cases xa_yb; rename_i xa yb
+  cases swap_s_t
+  rename_i swap_1 swap_23
+  cases swap_23
+  rename_i swap_2 swap_3
+  cases swap_1
+  cases swap_2
+  cases swap_3
+  simp [aval, upd, *]
+```
+
+
+
+
+
+
+
+
+
+
+
+
+
+Lets try to prove that `swap` indeed correctly swaps the values of `x` and `y`.
+
+How can we *specify* this correctness property as a theorem?
+
+How can we *prove* that theorem?
+
+<br>
+<br>
+<br>
+<br>
+<br>
+
+
+```lean
+theorem swap_swaps : ∀ {s t : State} {n m : Val},
+  s x = n -> s y = m -> (⟨ swap, s ⟩ ==> t) -> (t x = m) /\ (t y = n) := by
+```
+  intros s t n m sxn sym swap_123
+  simp_all [swap]
+  cases swap_123; rename_i s1 swap_1 swap_23
+  cases swap_23; rename_i s2 swap_2 swap_3
+  cases swap_1; cases swap_2; cases swap_3
+  simp_all [aval, upd]
+
+
+Instead of the `cases` we can prove a theorem that precisely characterizes what the "shape"
+of output state of an assignment is:
+
+
+```lean
+-- @[simp]
+theorem assign_step : ∀ {x a s t}, (⟨ x <~ a, s ⟩ ==> t) <-> (t = (s [x := aval a s])) := by
+  intros x a s t
+  apply Iff.intro
+  . case mp => intros xs; cases xs ; trivial
+  . case mpr => intros; simp_all [] ; apply BigStep.Assign
+```
+
+
+And now, we can tell `lean` to use that `assign_step` to "fill in" the intermediate
+`s1`, `s2` and `s3` to complete the proof.
+
+```lean
+theorem swap_swaps' : ∀ {s t : State} {n m : Val},
+  s x = n -> s y = m -> (⟨ swap, s ⟩ ==> t) -> (t x = m) /\ (t y = n) := by
+  intros s t n m sxn sym swap_123
+  simp_all [swap]
+  cases swap_123; rename_i s1 swap_1 swap_23
+  cases swap_23; rename_i s2 swap_2 swap_3
+  simp_all [assign_step, aval, upd]
+```
+
+
+
+Well, that wasn't _too_ bad. But lets try a more interesting example:.
+
+## Example: Summing the numbers from 0..n
+
+Consider the following *loop* which sums up the values of the numbers from `0` to `x`
+
+
+∀ {start finish a},
+⟨ sum_com, start ⟩ ==> finish
+->
+start x = a
+->
+finish y = sumTo a
+
+start
+  x = a
+finish
+  y = sumTo a
+
+
+```lean
+def sumTo (n: Nat) : Nat :=
+  match n with
+  | 0 => 0
+  | n' + 1 => n' + sumTo n'
+
+
+def sum_com : Com :=
+-- {{ x = a }}
+  y <~ 0 ;;
+-- {{ x = a /\ y = 0 }}
+   WHILE
+--   {{ x <= a }}
+     0 << x
+   DO
+--   {{ x <= a /\ 0 < x }}
+    y <~ y + x ;;
+    x <~ x - 1
+  END
+
+-- {{ y = sum a }}
+
+-- x = a, y = 0
+-- x = a-1, y=a
+-- x = a-2, y=a + a -1
+-- x = a-3, y=a + a - 1 + a - 2
+-- x = 0  , y= a + a-1 + a-2 + ... + 1
+-- y = 1 + 2 + 3 + ... + a
+```
+
+How can we **specify** that this correctly sums up the numbers `0 + ... + n` ?
+
+<br>
+<br>
+<br>
+<br>
+<br>
+
+
+
+```lean
+def sum (n:Nat) : Nat :=
+  match n with
+    | 0      => 0
+    | n' + 1 => n + sum n'
+
+-- A program! ------------------------------------------------------------
+
+abbrev csum := y <~ y + x ;; x <~ x - 1
+abbrev wsum := WHILE 0 << x DO csum END
+abbrev imp_sum := "y" <~ 0 ;; wsum
+
+theorem wsum_sum' : (⟨ wsum, s ⟩ ==> t) -> ((t "y") = s "y" + sum (s "x")) := by
+  sorry
+  -- intro wsum_s_t
+  -- generalize h : wsum = ws at wsum_s_t -- LEAN:ANF BUG
+  -- induction wsum_s_t <;> simp_all [wsum]
+  -- . case WhileFalse =>
+  --   cases h
+  --   rename_i c _ s bfalse left _
+  --   simp [<-left] at bfalse
+  --   simp_all [bval, aval, sum]
+  -- . case WhileTrue =>
+  --   cases h
+  --   rename_i b c s s1 t btrue c_s_s1 w_s1_t left right
+  --   simp [<-left] at btrue
+  --   sorry
+
+
+
+theorem csum_sum : (⟨ csum, s ⟩ ==> t) -> ( (t "x" = s "x" - 1) /\ (t "y") = s "y" + s "x")
+  := by
+  intros cs; cases cs; rename_i s1 st1 st2; simp_all [assign_step]
+  by_cases (x=y) <;> (simp_all [upd, aval]; try intros; contradiction)
+
+theorem wsum_sum : (⟨ wsum, s ⟩ ==> t) -> ((t "y") = s "y" + sum (s "x")) := by
+  intros wsums
+  generalize h : wsum = ws at wsums -- LEAN:ANF BUG
+  induction wsums <;> try simp_all []
+  .case WhileFalse =>
+   cases h
+   rename_i b c s bfalse cond _
+   have x_eq_0 : s "x" = 0 := by
+     simp [<-cond, bval, aval] at bfalse
+     assumption
+   simp_all [sum]
+  .case WhileTrue =>
+    rename_i b csum s s1 s2 btrue c_step _ _ _
+    cases h
+    rename_i cond hr
+    have s1xy : s1 "x" = s "x" - 1 /\ s1 "y" = s "y" + s "x" := by
+      apply csum_sum; simp_all []
+    cases s1xy
+    have sum_x : sum (s "x") = s "x" + sum (s "x" - 1) := by
+      simp [<-cond, bval, aval] at btrue
+      generalize hx : s "x" = sx
+      cases sx <;> simp_all [sum]
+    simp_all [Nat.add_assoc]
+
+theorem while_sum : (⟨ imp_sum, s ⟩ ==> t) -> t "y" = sum (s "x") := by
+  intros ws
+  cases ws
+  rename_i y0_step ws_step
+  cases y0_step
+  generalize h : upd s y (aval 0 s) = s0 at ws_step
+  have hyp  : ((t "y") = s0 "y" + sum (s0 "x")) := by apply wsum_sum; simp_all [<-h]
+  have h0   : s0 "y" = 0 := by simp_all [<-h, upd, aval]
+  have s0_x : s0 "x" = s "x" := by simp_all [<-h, upd]
+  simp_all []
+```
+
+
+Yikes, that was like pulling teeth. Lets look at a better way, introduced by
+Robert Floyd, back in 1967 (using the same example!)
+
+![Assigning meaning to programs](../static/floyd-sum.png)
+
+Floyd's paper formulated everything for **flow-charts**
+
+In 1969 Tony Hoare reformulated those ideas as
+
+![An Axiomatic Basis for Programming](../static/hoare-axiomatic.png)
+
+which is what we today call **axiomatic semantics** or **Floyd-Hoare (FH) Logic**.
+
+## Assertions
+
+The *central* idea in FH logic is the notion of an **assertion** which is simply property of a `State`,
+that is some **fact** that is true (or not) about a particular program `State`.
+
+
+```lean
+abbrev Assertion := State -> Prop
+```
+
+For example, the state `s` defined as `s0 [x := 10] [ y := 20]` satisfies the following assertions
+
+- `λ s -> s x < s y`
+- `λ s -> s x + s y = 30`
+
+but *does not* satisfy the assertions
+
+- `λ s -> s x = 0`
+- `λ s -> s x > s y`
+
+## Floyd-Hoare Triples
+
+A Floyd-Hoare **triple** is a `{{ p }} c {{ q }}` where
+
+- `p` is a **pre-condition** assertion,
+- `c` is a **command**, and
+- `q` is a **post-condition**.
+
+Intuitively, the triple `{{ p }} c {{ q }}` says that
+
+**If**
+- the command `c` is executed from a state where the _precondition_ `p` holds and
+- the execution of `c` _terminates_,
+
+**Then**
+- upon termination, the _postcondition_ `q` will hold.
+
+We can state the above precisely by defining when a triple is *valid*
+
+
+```lean
+@[simp]
+def Valid (p: Assertion) (c: Com) (q: Assertion) :=
+  ∀ s t, p s -> (⟨ c, s ⟩ ==> t) -> q t
+
+notation:10 "⊧" " {{" p "}} " c " {{" q "}}" => Valid p c q
+```
+
+## Example: Correctness of `imp_sum`
+
+We can restate the correctness of `imp_sum` as a FH triple as
+
+
+    { p } SKIP    { p }
+
+
+    { q [[ x := a ]] } x <~ a  { q }
+
+
+    { a > 15  } x <~ a  { x > 15 }
+
+
+
+```lean
+example : ∀ {n},
+  ⊧ {{ fun s => s "x" = n }} imp_sum {{ fun t => t "y" = sum n }}
+  := by
+  simp_all []
+  intros n s t xn imp_step
+  simp_all [<-xn]
+  apply while_sum
+  trivial
+```
+
+
+## Floyd-Hoare Logic
+
+The notion of a *valid triple* is useful in defining a *specification* of correctness,
+but we still have to go through the painful and quite tedious proof of `while_sum` to
+actually *verify* the triple.
+
+### Proof Rules
+
+The really clever contribution of Floyd and Hoare was to come up with a **recipe**
+comprising a system of **proof rules** that can be **automatically** applied to do
+the verification, without *ever* directly using the big-step semantics!
+
+These rules are **compositional** meaning that we derive the triple `{P} c {Q}`
+by using sub-derivations on the sub-commands of `c`.
+
+
+### Rule: Skip
+
+For example, we have a rule for the `Skip` command that says
+
+```
+---------------- [skip]
+⊢ {P} SKIP {P}
+```
+
+That is, for *any* assertion `p` we can derive that if `p` holds _before_ the `SKIP`
+then it must hold _after_ as well.
+
+### Rule: Sequence
+
+The rule for sequencing two commands `c1; c2` says that
+
+```
+⊢ {p} c1 {q}      ⊢ {q} c2 {r}
+--------------------------------[seq]
+⊢ {p} c1; c2 {r}
+```
+
+That is, `⊢ {p} c1; c2 {r}` holds if
+
+1. there is some *intermediate assertion* `q`
+2. that holds after executing `c1` from a `{p}` state, and
+3. `c2` then takes all `q` states to `r` states.
+
+### Rule: Assignment
+
+The rule for assignment is quite tricky.
+
+When *can* we be sure that some assertion `q` holds *after* executing `x <~ a` ?
+
+Lets look at some examples to build up some intuition.
+
+What assertion can you write for `???` in each of the below?
+
+- `{???} x <~ 10  { x > 0 }`
+
+- `{???} x <~ y   { x > 0 }`
+
+- `{???} x <~ a+b { x + a > 0 }`
+
+Can you spot some sort of a **pattern**?
+
+Indeed, if we want `q` to be true *after* the assignment `x <~ a` then
+
+1. The _only_ change made by the assignment is to `x`
+
+2. So it must be that `q` is true _before_ the assignment
+
+3. Except with all occurences of `x` (in `q`) replaced with `a` !
+
+### Example: `Swap`
+
+Lets see how the rules for assignment and sequence work for our `swap` example from above.
+
+```
+{{ s y = b /\ s x = a }}
+
+  z <~ var x ;;
+
+{{ s y = b /\ s z = a }}
+
+  x <~ var y ;;
+
+{{ s x = b /\ s z = a }}
+
+  y <~ var z
+
+{{ s x = b /\ s y = a }}
+```
+
+### Rule: If-Then-Else
+
+Lets try to work out the rule for establishing
+a triple `⊢ {p} IF cond THEN c1 ELSE c2 {q}`.
+
+Lets think about this triple:
+
+```
+{ ??? }
+
+  IF 0 < x
+
+    THEN y <~ x
+
+    ELSE y <~ 0 - x
+
+{ 0 <= y }
+```
+
+What must be true _before_ the IF-THEN-ELSE
+so that we can be sure that `0 <= y` _after_?
+
+How can we know that the above triple holds?
+
+Can you think of the appropriate triples that
+must hold for `c1` and `c2` ? How about the rule
+
+```
+⊢ {P} c1 {Q}    ⊢ {P} c2 {Q}
+-------------------------------- [If]
+⊢ {P} IF b THEN c1 ELSE c2 {Q}
+```
+
+Is it "sound" (does it **prove invalid triples** ?)
+
+Is it "complete" (does it **prevent proving valid triples?**)
+
+How can we fix the rule?
+
+```
+⊢ {???} c1 {Q}    ⊢ { ??? } c2 {Q}
+------------------------------------ [If]
+⊢ {P} IF b THEN c1 ELSE c2 {Q}
+```
+
+Lets go back to the example
+
+
+```
+⊢ {true /\ 0 < x} y <~ x { 0 <= y }   ⊢ {true /\ ¬ 0 < x} y <~ 0 - x { 0 <= y }
+-------------------------------------------------------------------------------- [If]
+⊢ { true } IF (0 < x) THEN y <~ x ELSE y <~ 0 - x) { 0 <= y }
+```
+
+
+### FH rules are too "tight"
+
+
+Consider this triple: _surely_ it should be valid but we
+cannot *prove* it with our rules :-(
+
+```
+{x = 10} SKIP { x > 0}          (ex1)
+```
+
+The skip rule will let us prove that
+
+```
+⊢ {x=10} SKIP {x=10}
+```
+
+and that
+
+```
+⊢ {x > 0} SKIP {x > 0}
+```
+
+but surely we should _also_ be able to prove `{x=10} SKIP {x>0}`?
+
+Here's another example.
+
+```
+{x = 0} x <~ x + 1 {x = 1}      (ex2)
+```
+
+The `Assign` rule will let us prove that `{x+1 = 1} x <~ x + 1 {x = 1}` but
+not directly that `{x=0} x <~ x + 1 {x=1}` ... which seems silly!
+
+Can you think about *why* the above triples `ex1` and `ex2`  hold?
+
+### Bonus Rule: Consequence
+
+How can we encode the above intuition as a *rule*?
+
+<br>
+<br>
+<br>
+<br>
+<br>
+<br>
+<br>
+<br>
+<br>
+<br>
+
+We can *relax* the FH rules with the **rule of consequence** shown below.
+
+```
+∀ s. P(s) => P'(s)    ⊢ {P'} c {Q'}     ∀ s. Q'(s) => Q(s)
+----------------------------------------------------------- [Consequence]
+⊢ {P} c {Q}
+```
+
+This rule says that
+
+- if you can establish the triple `⊢ {P'} c {Q'}` then
+
+![After you establish a triple...](static/fh_conseq_1.png)
+
+- you can **strengthen the precondition** meaning, that if `⊢ {P'} c {Q'}` holds
+  then you can replace the `P'` with any assertion `P` that is
+  **stronger than** `P'` i.e. whenever `P` is true, `P'` is *also* true, and
+
+![Strengthening the Precondition](../static/fh_conseq_2.png)
+
+- you can **weaken the postcondition** meaning, that if `⊢ {P'} c {Q'}` holds
+  then you can replace the `Q'` with any assertion `Q` that is
+  **weaker than** `Q'` i.e. whenever `Q'` is true, then `Q` is *also* true.
+
+![Weakening the Postcondition](../static/fh_conseq_2.png)
+
+So, for example, we can do
+
+
+```
+--------------------[skip]
+⊢ {x=10} SKIP {x=10}              x=10 => x>0
+---------------------------------------------[conseq]
+⊢ {x=10} SKIP {x>0}
+
+
+                    ------------------[skip]
+x=10 => x>0         ⊢ {x>0} SKIP {x>0}
+--------------------------------------------[conseq]
+⊢ {x=10} SKIP {x>0}
+
+
+                   --------------------------[assign]
+x=0 => x+1=1       ⊢ {x+1=1} x <~ x + 1 {x=1}
+---------------------------------------------[conseq]
+⊢ {x=0} x <~ x + 1 {x=1}
+```
+
+### Rule: While
+
+Did we forget something: what about `WHILE` loops?
+
+Lets pick a simple example. How can we prove that after executing the loop below,
+the value of `x` is non-negative?
+
+```
+{{ True }}
+
+  i <~ 0;
+
+  x <~ 0;
+
+  WHILE (i <= n) DO
+
+    x <~ x + i;;
+
+    i <~ i - 1
+
+  DONE
+
+{{ 0 <= x }}
+```
+
+**Loop Invariants**
+We need a way to describe an assertion that is true,
+no matter how many times the loop runs. Such an assertion
+is called a *loop invariant*. As the name suggests, the
+invariant must be true
+
+- **base case** before the loop starts executing,
+- **inductive case** if the invariant holds _before_ one iteration, it must hold _after_ an iteration.
+
+Lets try to fill in the blanks in the rule below!
+
+```
+⊢ {???} c {???}
+-------------------------------- [while]
+⊢ {???} WHILE b DO c DONE {???}
+```
+
+When we're done, we should be able to prove (what is the magic `I`) ?
+
+```
+{true} i <~ 0;; x <~ 0;; WHILE i <= n DO (x <~ x+i;;i<~ i-1) DONE {0<=x}`
+```
+
+### Example: `sum`
+
+```
+{{ x = i /\ 0 <= i }}
+=>
+{{ 0 + sum x = sum i /\ 0 <= i }}
+  y <~ 0
+{{ y + sum x = sum i /\ 0 <= i}}
+
+WHILE (0 < x) DO
+  {{ y + sum x = sum i /\ 0 <= x }}
+  y <~ y + x
+  x <~ x - 1
+
+{{ ¬ 0 < x /\ y + sum x = sum i /\ 0 <= x }}
+=>
+{{ y = sum i}}
+```
+
+## Formalizing the Floyd-Hoare Rules
+
+It is pretty straightforward to formalize the FH rules
+as an inductive predicate in `lean`.
+
+### Formalizing Implication `⊆`
+
+First, we need to define implication
+
+
+```lean
+open Com
+
+@[simp]
+def Implies (p q : Assertion) := ∀ s, p s -> q s
+
+notation:10 p " ⊆ " q => Implies p q
+```
+
+Let us define the assertions `tt` ("true") and `ff` ("false") as
+
+```lean
+@[simp]
+def tt : Assertion := fun _ => True
+
+@[simp]
+def ff : Assertion := fun _ => False
+```
+
+Now, we can easily prove the following implications, e.g.
+
+```lean
+theorem p_imp_true  : ∀ {p : Assertion}, p ⊆ tt := by
+  simp []
+
+theorem false_imp_p : ∀ {p : Assertion}, ff ⊆ p := by
+  simp []
+
+example : (λ s => s x = 10) ⊆ (λ s => s x > 0 ) := by
+  intros s x_10
+  simp_all []
+```
+
+
+### Formalizing Substitution
+
+Next, lets formalize the idea of "substitution" as appears in the `Assign` rule.
+
+```
+⊢ { Q[x := a] } x <~ a { Q }
+```
+
+What, exactly, does it mean for `Q` to hold with the value of `x` replaced by `a` ?
+
+
+```lean
+notation:10 p "[[ " x ":=" a "]]" => fun s => p (s [ x := (aval a s) ])
+```
+
+
+Lets go and revisit our examples from above:
+
+**NOTE** The `funext s` tactic lets us prove two functions are equal by proving
+they produce the same (equal) result on all inputs `s`.
+
+```lean
+-- 1. `{true} x <~ 10  { 0 < x }`
+example : ((λ s => 0 < s x) [[ x := 10 ]]) = tt := by
+  funext
+  simp [aval, upd]
+
+-- 2. `{0 < y} x <~ y  {0 < x}`
+example : ((λ s => 0 < s x) [[ x := var y ]]) = (λ s => 0 < s y) := by
+  funext
+  simp [aval, upd]
+
+theorem implies_refl : ∀ p, p ⊆ p := by
+  intro p s h
+  assumption
+```
+
+
+### Formalizing The Proof Rules
+
+
+
+```lean
+inductive FH : Assertion -> Com -> Assertion -> Prop where
+
+  | Skip              : ∀ {p},
+                          FH p Skip p
+
+  | Assign            : ∀ {p x a},
+                          FH (p [[ x := a ]]) (x <~ a) p
+
+  | Seq               : ∀ {p c1 c2 q r},
+                          FH p c1 q -> FH q c2 r ->
+                          FH p (c1 ;; c2) r
+
+  | If                : ∀ {p b c1 c2 q},
+                        FH (fun s => p s /\   bval b s) c1 q -> FH (fun s => p s /\ ¬ bval b s) c2 q ->
+                        FH p (If b c1 c2) q
+
+  | While             : ∀ {p b c},
+                        FH (fun s => p s /\ bval b s) c p ->
+                        FH p (While b c) (fun s => p s /\ ¬ bval b s)
+
+  -- | Cnsq              : ∀ {p' p c q q'},
+  --                       (p' ⊆ p) -> FH p c q -> (q ⊆ q') ->
+  --                       FH p' c q'
+  | CnsL              : ∀ {p' p c q},
+                        FH p c q ->
+                        (p' ⊆ p) ->
+                        FH p' c q
+  | CnsR              : ∀ {p c q q'},
+                        FH p c q ->
+                        (q ⊆ q') ->
+                        FH p c q'
+
+notation:10 "⊢" " {{" p "}} " c " {{" q "}}" => FH p c q
+```
+
+## Examples, Mechanized
+
+### Swap
+
+Recall the informal proof of `swap` above
+
+```
+{{ y = b /\ x = a }}    p
+
+  z <~ var x ;;
+
+{{ y = b /\ z = a }}    p0
+
+  x <~ var y ;;
+
+{{ x = b /\ z = a }}    p1
+
+  y <~ var z
+
+{{ x = b /\ y = a }}    q
+```
+
+Lets formally prove the above using the FH rules. (Yuck, still gross!)
+
+
+```lean
+theorem swap_correct : ∀ {a b : Val},
+  ⊢ {{ λ s => (s y = b /\ s x = a) }}
+    swap
+    {{ λ s => (s x = b /\ s y = a) }}
+  := by
+  intros a b
+  generalize hp  : (λ (s: State) => (s y = b /\ s x = a)) = p
+  generalize hp0 : (λ (s: State) => (s y = b /\ s z = a)) = p0
+  generalize hp1 : (λ (s: State) => (s x = b /\ s z = a)) = p1
+  generalize hq  : (λ (s: State) => (s x = b /\ s y = a)) = q
+  have s0 : ⊢ {{ p }}  z <~ var x {{ p0 }} := by
+    simp [<-hp, <-hp0]
+    apply FH.CnsL; apply FH.Assign; simp [aval,upd]
+  have s1 : ⊢ {{ p0 }} x <~ var y {{ p1 }} := by
+    simp [<-hp0, <-hp1]
+    apply FH.CnsL; apply FH.Assign; simp [aval,upd]
+  have s2 : ⊢ {{ p1 }} y <~ var z {{ q  }} := by
+    simp [<-hp1, <-hq]; apply FH.CnsL; apply FH.Assign; simp [aval,upd]
+  simp [swap]
+  constructor
+  assumption
+  constructor
+  assumption
+  assumption
+```
+
+
+### Loop
+
+Recall the informal proof of `loop` above
+
+```
+{{ True }}
+
+  i <~ 0;
+
+  x <~ 0;
+
+  WHILE (i <= n) DO
+
+    x <~ x + i;;
+
+    i <~ i - 1
+
+  DONE
+
+{{ 0 <= x }}
+```
+
+**EXERCISE:** Formally prove the above using the FH rules.
+
+### Sum
+
+Finally,
+
+```
+{{ x = i /\ 0 <= i }}
+=>
+{{ 0 + sum x = sum i /\ 0 <= i }}
+  y <~ 0
+{{ y + sum x = sum i /\ 0 <= i}}
+
+WHILE (0 < x) DO
+  {{ y + sum x = sum i /\ 0 <= x }}
+  y <~ y + x
+  x <~ x - 1
+
+{{ ¬ 0 < x /\ y + sum x = sum i /\ 0 <= x }}
+=>
+{{ y = sum i}}
+```
+
+```lean
+def wsum_inv (i:Nat) : Assertion := λ s => s "y" + sum (s "x") = sum i
+
+theorem y0_fh : ⊢ {{λ s => s x = i }} (y <~ 0) {{wsum_inv i }} := by
+  generalize h' : (λ (s:State) => s x = i)  = p'
+  generalize h  : (wsum_inv i [[ y := 0 ]]) = p
+  have aa : p' ⊆ p := by simp_all [<-h', <-h, Implies, wsum_inv, upd, aval]
+  have bb : ⊢  {{ p }}  (y <~ 0) {{wsum_inv i }} := by simp [<-h]; apply FH.Assign
+  apply FH.CnsL
+  assumption
+  assumption
+
+theorem csum_fh : ⊢ {{λ s => wsum_inv i s /\ (bval (0 << "x") s)}} csum {{wsum_inv i }} := by
+  generalize h1 : (wsum_inv i [[ x := x - 1 ]]) = q1
+  generalize h2 : (q1 [[ y := y + x ]])         = q2
+  have c1   : ⊢ {{ q1 }} x <~ x - 1 {{wsum_inv i }} := by simp_all [<-h1]; apply FH.Assign
+  have c2   : ⊢ {{ q2 }} y <~ y + x {{ q1 }}        := by simp_all [<-h2]; apply FH.Assign
+  have c12  : ⊢ {{ q2 }} csum {{wsum_inv i }}       := by apply FH.Seq; assumption; assumption
+  have imp1 : (λ s => wsum_inv i s /\ 0 < s x ) ⊆ q2 := by
+    simp_all [<-h2, <-h1, upd, Implies, bval, aval, wsum_inv]
+    by_cases (x = y) <;> simp_all []
+    .case neg =>
+      intros s h1 h2
+      generalize hx : s x = sx
+      cases sx <;> simp_all [sum, Nat.add_assoc]
+  apply FH.CnsL
+  apply c12
+  simp_all [bval, aval]
+
+theorem imp_sum_fh : ⊢ {{ λ s => s "x" = i }} imp_sum {{ λ s => s "y" = sum i }} := by
+  have wsum_fh : ⊢ {{wsum_inv i }} wsum {{ λs => wsum_inv i s /\ ¬ (bval (0 << x) s) }} := by
+    apply FH.While; apply csum_fh
+  have imp_sum' : ⊢ {{ λ s => s "x" = i }} imp_sum {{ λ s => wsum_inv i s /\ ¬ (bval (0 << "x") s)}} := by
+    apply FH.Seq; apply y0_fh; apply wsum_fh
+  have wsum_exit : (λ s => wsum_inv i s /\ ¬ (bval (0 << "x") s)) ⊆ (λ s => s "y" = sum i) := by
+    simp_all [wsum_inv, Implies, bval, aval, sum]; intros; simp_all [sum]
+  apply FH.CnsR
+  apply imp_sum'
+  apply wsum_exit
+```
+
+
+
+## Soundness of Floyd-Hoare Logic
+
+The great thing about formalizing the definition of `Validity` and the proof rules
+is that we can now *prove* that we did not just make stuff up.
+
+That is, we can prove that the Floyd-Hoare logic is **sound** meaning that if we
+can only **derive valid triples** in the logic. That is, if the proof rules let us
+conclude the triple `⊢ {{p}} c {{q}}` then that triple is in fact valid.
+
+
+```lean
+theorem while_exit : (⟨ WHILE b DO c END, s ⟩ ==> t) -> bval b t = false := by
+  intro h
+  generalize h' : (WHILE b DO c END) = c' at h
+  induction h <;> try simp_all []
+
+theorem loop_sound {p : Assertion} :
+  (∀ {s t}, (p s /\ bval b s = true) -> (⟨ c, s ⟩ ==> t) -> (p t)) ->
+  (⟨ WHILE b DO c END, s ⟩ ==> t) ->
+  p s ->
+  p t := by
+  intros inv step ps
+  generalize bob : (WHILE b DO c END) = wbc at step
+  induction step <;> simp_all []
+  rename_i ih
+  apply ih
+  apply inv
+  apply ps
+  assumption
+  assumption
+
+theorem fh_sound :  ( ⊢ {{ p }} c {{ q }} ) -> ( ⊧ {{ p }} c {{ q }} )  := by
+  simp_all [Valid]
+  intro h s t ps step
+  induction h generalizing s t
+  . case Skip   => rename_i step ; cases step; assumption
+  . case Assign => intros; rename_i step ; cases step; assumption
+  . case Seq    => intros; rename_i ih1 ih2; cases step; apply ih2; apply ih1; repeat assumption
+  . case If =>
+    intros; rename_i ih1 ih2; cases step <;> simp_all []
+    . case IfTrue => apply ih1; repeat assumption
+    . case IfFalse => apply ih2; assumption; simp_all []; assumption
+  . case While =>
+    rename_i b c _ ih
+    generalize hh : (WHILE b DO c END) = wbc at step
+    apply And.intro
+    apply loop_sound
+    assumption
+    simp_all []
+    assumption
+    assumption
+    have bf : bval b t = false := by
+      apply while_exit
+      simp [<- hh] at step
+      apply step
+    simp_all []
+  . case CnsL =>
+    rename_i p' _ c _ _ p'p ih
+    apply ih; apply p'p; repeat assumption
+
+  . case CnsR =>
+    rename_i p c _ _ _ qq' ih
+    apply qq'; apply ih; repeat assumption
+```
+
+
+To recap: the Floyd-Hoare rules give us a sound way to construct proofs of programs,
+but, lets be honest, the construction is a real PITA.
+
+Next, lets see how to dramatically automate these proofs using **verification conditions**.
+
+
